verifier/src/main/resources/additional.dfy
@@ -9,7 +9,11 @@ type int64 = x: int | -0x8000_0000_0000_0000 <= x <= 0x7fff_ffff_ffff_ffff
 
 // Base type is int and not char, because Java's char allows surrogates and Dafny's char does not
 type char16 = i: int | 0x0000 <= i <= 0xffff
-type jstring = seq<char16>
+newtype jstring extends Object = seq<char16> {
+  predicate equals(other: Object) {
+    other is jstring && this == (other as jstring)
+  }
+}
 
 function JString(s: string): jstring
   requires forall i | 0 <= i < |s| :: 0x0000 <= s[i] as int <= 0xffff
